type unification scaffold

Spacetalk/Step.lean
@@ -1,45 +1,53 @@
 import Spacetalk.Stream
 import Spacetalk.HList
+import Spacetalk.Graph
 
 -- Source Lang
 namespace Step
 
 ------------------ Syntax ------------------
-inductive Prim
-  | bitVec : Nat → Prim
-  deriving DecidableEq
-
-@[reducible]
-def Prim.denote : Prim → Type
-  | bitVec w => BitVec w
-
 inductive Ty
-  | stream : Prim → Ty
+  | bitVec : Nat → Ty
   deriving DecidableEq
-
-@[simp]
-def Ty.prim : Ty → Prim
-  | stream p => p
 
 @[reducible]
 def Ty.denote : Ty → Type
-  | stream p => Stream' p.denote
+  | bitVec w => BitVec w
 
-abbrev TysInput (tys : List Ty) := HList Ty.denote tys
+def Ty.default : (ty : Ty) → ty.denote
+  | bitVec _ => 0
 
-inductive BinaryOp : Prim → Prim → Prim → Type
+instance : Denote Ty where
+  denote := Ty.denote
+  default := Ty.default
+
+-- inductive Ty
+--   | stream : Prim → Ty
+--   deriving DecidableEq
+
+-- @[simp]
+-- def Ty.prim : Ty → Prim
+--   | stream p => p
+
+-- @[reducible]
+-- def Ty.denote : Ty → Type
+  -- | stream p => Stream' p.denote
+
+-- abbrev TysInput (tys : List Ty) := HList Ty.denote tys
+
+inductive BinaryOp : Ty → Ty → Ty → Type
   | add : {w : Nat} → BinaryOp (.bitVec w) (.bitVec w) (.bitVec w)
   | mul : {w : Nat} → BinaryOp (.bitVec w) (.bitVec w) (.bitVec w)
 
-inductive UnaryOp : Prim → Prim → Type
+inductive UnaryOp : Ty → Ty → Type
   | addConst : {w : Nat} → BitVec w → UnaryOp (.bitVec w) (.bitVec w)
   | mulConst : {w : Nat} → BitVec w → UnaryOp (.bitVec w) (.bitVec w)
 
 inductive Prog : List Ty → Ty → Type
   | const : (α : Ty) → Prog [α] α
-  | zip : BinaryOp α β γ → Prog aInp (.stream α) → Prog bInp (.stream β) → Prog (aInp ++ bInp) (.stream γ)
-  | map : UnaryOp α β → Prog inp (.stream α) → Prog inp (.stream β)
-  | reduce : BinaryOp α β α → Nat → α.denote → Prog inp (.stream β) → Prog inp (.stream α)
+  | zip : BinaryOp α β γ → Prog aInp α → Prog bInp β → Prog (aInp ++ bInp) γ
+  | map : UnaryOp α β → Prog inp α → Prog inp β
+  | reduce : BinaryOp α β α → Nat → α.denote → Prog inp β → Prog inp α
 
 ------------------ Semantics ------------------
 def BinaryOp.denote : BinaryOp α β γ → α.denote → β.denote → γ.denote
@@ -50,7 +58,7 @@ def UnaryOp.denote : UnaryOp α β → α.denote → β.denote
   | UnaryOp.addConst c => BitVec.add c
   | UnaryOp.mulConst c => BitVec.mul c
 
-def Prog.denote {inputs : List Ty} {α : Ty} : Prog inputs α → (TysInput inputs → TysInput [α])
+def Prog.denote {inputs : List Ty} {α : Ty} : Prog inputs α → (DenoStreamsList inputs → DenoStreamsList [α])
   | .const _ => λ ([a]ₕ) ↦ [a]ₕ
   | .zip op as bs => λ inp ↦ let (aInp, bInp) := inp.split; [Stream'.zip op.denote (as.denote aInp).head (bs.denote bInp).head]ₕ
   | .map op as => λ inp ↦ [Stream'.map op.denote (as.denote inp).head]ₕ
